\begin{table}
	[htbp] 
	\begin{center}
		\begin{tabular}
			{p{\myTableWidth}p{\myTableWidth}} \toprule $ \mu = 3.986005 \times 10^{14}~\text{m}^3/\text{s}^2 $ & Earth’ universal gravitational parameter\\\midrule
			$ \Omega_e = 7.2921151467 \times 10^{-5}~\text{rad}/\text{s} $ & Earth’ rotation rate \\ \midrule
			$ A=(\sqrt{A})^2 $ & Semi-major axis \\ \midrule
			$ n=\sqrt{\frac{\mu}{A^3}} $ & Computed mean motion  \\ \midrule
			$t_k = t^s - t_{oe }$ 
			\begin{equation*}
				t_k = 
				\begin{cases}
					 t_k -604800 , &\text{ if }t_k> 302400\\
					 t_k +604800 , &\text{ if }t_k< -302400\\
					 t_k		 , &\text{ otherwise }
				\end{cases}
			\end{equation*}
			 & {\multirow{5}{*}{Time from ephemeris reference epoch}}\\\midrule
			$ n=n_0 +\Delta n $ & Corrected mean motion \\ \midrule
			$ M_k =M_0 +nt_k $ & Mean anomaly \\ \midrule
			$ E_k =M_k +e\sin E_k $ & Kepler’s equation for eccentric anomaly. Solution by Eq. (23) \\ \midrule
			$ \sin \nu_k = (\sqrt{1-e^2} \sin E_k)/(1-e\cos E_k) $ &{\multirow{2}{*}{True Anomoly} }	 \\ 
			$ \cos \nu_k = (\cos E_k -e)/(1-e\cos E_k) $ & ~ \\ \midrule
			$ \Phi_k = \nu_k +\omega $ & Argument of latitude \\ \midrule
			$ \delta u_k =\text{c}_{us}\sin 2\Phi_k +c_{uc}\cos 2\Phi_k $ & Argument of latitude correction \\ \midrule
			$ \delta r_k =\text{c}_{rs}\sin 2\Phi_k +c_{rc}\cos 2\Phi_k $ & Radius correction \\ \midrule
			$ \delta i_k =\text{c}_{is}\sin 2\Phi_k +c_{ic}\cos 2\Phi_k $ & Inclination correction \\ \midrule
			$ u_k =\Phi_k +\delta u_k $ & Corrected argument of latitude \\ \midrule
			$ r_k =A(1 - e\cos E_k)+\delta r_k $ & Corrected radius \\ \midrule
			$ i_k =i_0 +\delta i_k +(\text{IDOT})t_k $ & Corrected inclination \\ \midrule
			$ x'_k =r_k\cos u_k$ & {\multirow{2}{*}{Position in orbital plane}} \\ 
			$y'_k =r_k\sin u_k $ & ~ \\ \midrule
			$ \Omega_k =\Omega_0 +(\dot{\Omega}-\dot{\Omega}_e)t_k -\dot{\Omega}_{e}t_{oe} $ & Corrected longitude of ascending node \\ 
			$ x_k =x'_k \cos \Omega_k -y' \cos i \sin \Omega_k $ & WGS84 Cartesian coordinates, ($X^s = x_k$ \\ 
			$ y_k =x'_k \sin \Omega_k +y' \cos i \cos \Omega_k $ & $Y^s = y_k$, $Z^s = z_k$) \\ 
			$ z_k = y' \sin i_k $ & ~ \\ 
			\bottomrule 
		\end{tabular}
	\end{center}
	\caption{caption} 
\end{table}


